<?xml version="1.0"?>
<rdf:RDF xmlns="https://purls.helmholtz-metadaten.de/diso"
     xml:base="https://purls.helmholtz-metadaten.de/diso"
     xmlns:owl="http://www.w3.org/2002/07/owl#"
     xmlns:rdf="http://www.w3.org/1999/02/22-rdf-syntax-ns#"
     xmlns:xml="http://www.w3.org/XML/1998/namespace"
     xmlns:xsd="http://www.w3.org/2001/XMLSchema#"
     xmlns:rdfs="http://www.w3.org/2000/01/rdf-schema#"
     xmlns:vann="http://purl.org/vocab/vann/"
     xmlns:terms="http://purl.org/dc/terms/">
    <owl:Ontology rdf:about="https://purls.helmholtz-metadaten.de/diso">
        <terms:contributor rdf:datatype="http://www.w3.org/2001/XMLSchema#string">Said Fathalla</terms:contributor>
        <terms:contributor rdf:datatype="http://www.w3.org/2001/XMLSchema#string">Stefan Sandfeld</terms:contributor>
        <terms:created xml:lang="en">21.03.2022</terms:created>
        <terms:creator xml:lang="en">Ahmad Zainul Ihsan</terms:creator>
        <terms:title xml:lang="en">Dislocation Ontology</terms:title>
        <vann:preferredNamespacePrefix rdf:datatype="http://www.w3.org/2001/XMLSchema#string">DISO</vann:preferredNamespacePrefix>
        <rdfs:seeAlso>https://github.com/Materials-Data-Science-and-Informatics/dislocation-ontology</rdfs:seeAlso>
    </owl:Ontology>
    


    <!-- 
    ///////////////////////////////////////////////////////////////////////////////////////
    //
    // Annotation properties
    //
    ///////////////////////////////////////////////////////////////////////////////////////
     -->

    


    <!-- http://purl.org/dc/terms/contributor -->

    <owl:AnnotationProperty rdf:about="http://purl.org/dc/terms/contributor"/>
    


    <!-- http://purl.org/dc/terms/created -->

    <owl:AnnotationProperty rdf:about="http://purl.org/dc/terms/created"/>
    


    <!-- http://purl.org/dc/terms/creator -->

    <owl:AnnotationProperty rdf:about="http://purl.org/dc/terms/creator"/>
    


    <!-- http://purl.org/dc/terms/title -->

    <owl:AnnotationProperty rdf:about="http://purl.org/dc/terms/title"/>
    


    <!-- http://purl.org/vocab/vann/preferredNamespacePrefix -->

    <owl:AnnotationProperty rdf:about="http://purl.org/vocab/vann/preferredNamespacePrefix"/>
    


    <!-- 
    ///////////////////////////////////////////////////////////////////////////////////////
    //
    // Object Properties
    //
    ///////////////////////////////////////////////////////////////////////////////////////
     -->

    


    <!-- https://purls.helmholtz-metadaten.de/diso#hasBurgersVector -->

    <owl:ObjectProperty rdf:about="https://purls.helmholtz-metadaten.de/diso#hasBurgersVector">
        <rdfs:domain rdf:resource="https://purls.helmholtz-metadaten.de/diso#Dislocation"/>
        <rdfs:range rdf:resource="https://purls.helmholtz-metadaten.de/diso#BurgersVector"/>
        <rdfs:comment xml:lang="en">Representas relation from dislocation to Burgers vector</rdfs:comment>
        <rdfs:label xml:lang="en">has Burgers vector</rdfs:label>
    </owl:ObjectProperty>
    


    <!-- https://purls.helmholtz-metadaten.de/diso#hasEndNode -->

    <owl:ObjectProperty rdf:about="https://purls.helmholtz-metadaten.de/diso#hasEndNode">
        <rdfs:subPropertyOf rdf:resource="https://purls.helmholtz-metadaten.de/diso#hasNode"/>
        <rdfs:domain rdf:resource="https://purls.helmholtz-metadaten.de/diso#Segment"/>
        <rdfs:range rdf:resource="https://purls.helmholtz-metadaten.de/diso#Node"/>
        <rdfs:comment xml:lang="en">Sub-property of hasNode that relates the segment with the end node</rdfs:comment>
        <rdfs:label xml:lang="en">has end node</rdfs:label>
    </owl:ObjectProperty>
    


    <!-- https://purls.helmholtz-metadaten.de/diso#hasFamilyCrystalDirection -->

    <owl:ObjectProperty rdf:about="https://purls.helmholtz-metadaten.de/diso#hasFamilyCrystalDirection">
        <rdfs:domain rdf:resource="https://purls.helmholtz-metadaten.de/diso#LatticeDirection"/>
        <rdfs:range rdf:resource="https://purls.helmholtz-metadaten.de/diso#FamilyOfCrystalDirection"/>
        <rdfs:comment xml:lang="en">hasFamilyCrystalDirection represents the relationship between lattice direction and family of crystal direction.</rdfs:comment>
        <rdfs:label xml:lang="en">has family crystal direction</rdfs:label>
    </owl:ObjectProperty>
    


    <!-- https://purls.helmholtz-metadaten.de/diso#hasFamilyCrystalPlane -->

    <owl:ObjectProperty rdf:about="https://purls.helmholtz-metadaten.de/diso#hasFamilyCrystalPlane">
        <rdfs:domain rdf:resource="https://purls.helmholtz-metadaten.de/diso#LatticePlane"/>
        <rdfs:range rdf:resource="https://purls.helmholtz-metadaten.de/diso#FamilyOfCrystalPlane"/>
        <rdfs:comment xml:lang="en">hasFamilyCrystalPlane represents the relationship between lattice Plane and family of crystal plane.</rdfs:comment>
        <rdfs:label xml:lang="en">has family crystal plane</rdfs:label>
    </owl:ObjectProperty>
    


    <!-- https://purls.helmholtz-metadaten.de/diso#hasLatticeDirection -->

    <owl:ObjectProperty rdf:about="https://purls.helmholtz-metadaten.de/diso#hasLatticeDirection">
        <rdfs:range rdf:resource="https://purls.helmholtz-metadaten.de/diso#LatticeDirection"/>
        <rdfs:comment xml:lang="en">hasLatticeDirection represents the relationship between a lattice or a lattice plane and lattice directions.</rdfs:comment>
        <rdfs:label xml:lang="en">has lattice direction</rdfs:label>
    </owl:ObjectProperty>
    


    <!-- https://purls.helmholtz-metadaten.de/diso#hasLatticePlane -->

    <owl:ObjectProperty rdf:about="https://purls.helmholtz-metadaten.de/diso#hasLatticePlane">
        <rdfs:range rdf:resource="https://purls.helmholtz-metadaten.de/diso#LatticePlane"/>
        <rdfs:comment xml:lang="en">hasLatticePlane represents the relationship between a lattice and lattice planes.</rdfs:comment>
        <rdfs:label xml:lang="en">has lattice plane</rdfs:label>
    </owl:ObjectProperty>
    


    <!-- https://purls.helmholtz-metadaten.de/diso#hasLatticePoint -->

    <owl:ObjectProperty rdf:about="https://purls.helmholtz-metadaten.de/diso#hasLatticePoint">
        <rdfs:domain>
            <owl:Class>
                <owl:unionOf rdf:parseType="Collection">
                    <rdf:Description rdf:about="https://purls.helmholtz-metadaten.de/cso#Lattice"/>
                    <rdf:Description rdf:about="https://purls.helmholtz-metadaten.de/diso#LatticeDirection"/>
                    <rdf:Description rdf:about="https://purls.helmholtz-metadaten.de/diso#LatticePlane"/>
                </owl:unionOf>
            </owl:Class>
        </rdfs:domain>
        <rdfs:range rdf:resource="https://purls.helmholtz-metadaten.de/diso#LatticePoint"/>
        <rdfs:comment xml:lang="en">hasLatticePoint represents the relationship between a lattice or lattice plane or lattice direction with lattice points.</rdfs:comment>
        <rdfs:label xml:lang="en">has lattice point</rdfs:label>
    </owl:ObjectProperty>
    


    <!-- https://purls.helmholtz-metadaten.de/diso#hasLineSense -->

    <owl:ObjectProperty rdf:about="https://purls.helmholtz-metadaten.de/diso#hasLineSense">
        <rdfs:domain rdf:resource="https://purls.helmholtz-metadaten.de/diso#Dislocation"/>
        <rdfs:range rdf:resource="https://purls.helmholtz-metadaten.de/diso#LineSense"/>
        <rdfs:comment xml:lang="en">hasLineSense represents the relationship between a dislocation and a line sense.</rdfs:comment>
        <rdfs:label xml:lang="en">has line sense</rdfs:label>
    </owl:ObjectProperty>
    


    <!-- https://purls.helmholtz-metadaten.de/diso#hasMathematicalRepresentation -->

    <owl:ObjectProperty rdf:about="https://purls.helmholtz-metadaten.de/diso#hasMathematicalRepresentation">
        <rdfs:subPropertyOf rdf:resource="https://purls.helmholtz-metadaten.de/diso#hasRepresentation"/>
        <rdfs:comment xml:lang="en">relates the entity with its mathematical representation</rdfs:comment>
        <rdfs:label xml:lang="en">has mathematical representation</rdfs:label>
    </owl:ObjectProperty>
    


    <!-- https://purls.helmholtz-metadaten.de/diso#hasNode -->

    <owl:ObjectProperty rdf:about="https://purls.helmholtz-metadaten.de/diso#hasNode">
        <rdfs:domain rdf:resource="https://purls.helmholtz-metadaten.de/diso#Segment"/>
        <rdfs:range rdf:resource="https://purls.helmholtz-metadaten.de/diso#Node"/>
        <rdfs:comment xml:lang="en">hasNode represents the directed relation between segment and node</rdfs:comment>
        <rdfs:label xml:lang="en">has node</rdfs:label>
    </owl:ObjectProperty>
    


    <!-- https://purls.helmholtz-metadaten.de/diso#hasNumericalRepresentation -->

    <owl:ObjectProperty rdf:about="https://purls.helmholtz-metadaten.de/diso#hasNumericalRepresentation">
        <rdfs:subPropertyOf rdf:resource="https://purls.helmholtz-metadaten.de/diso#hasRepresentation"/>
        <rdfs:comment xml:lang="en">relates the entity with its numerical representation</rdfs:comment>
        <rdfs:label xml:lang="en">has numerical representation</rdfs:label>
    </owl:ObjectProperty>
    


    <!-- https://purls.helmholtz-metadaten.de/diso#hasOrigin -->

    <owl:ObjectProperty rdf:about="https://purls.helmholtz-metadaten.de/diso#hasOrigin">
        <rdfs:domain rdf:resource="https://purls.helmholtz-metadaten.de/diso#LatticePlane"/>
        <rdfs:range rdf:resource="https://purls.helmholtz-metadaten.de/diso#Origin"/>
        <rdfs:comment xml:lang="en">hasOrigin represents the directed relation between lattice plane and origin</rdfs:comment>
        <rdfs:label xml:lang="en">has origin</rdfs:label>
    </owl:ObjectProperty>
    


    <!-- https://purls.helmholtz-metadaten.de/diso#hasRepresentation -->

    <owl:ObjectProperty rdf:about="https://purls.helmholtz-metadaten.de/diso#hasRepresentation">
        <rdfs:comment xml:lang="en">has representation relates the entity to another representation of entity</rdfs:comment>
        <rdfs:label xml:lang="en">has representation</rdfs:label>
    </owl:ObjectProperty>
    


    <!-- https://purls.helmholtz-metadaten.de/diso#hasSegment -->

    <owl:ObjectProperty rdf:about="https://purls.helmholtz-metadaten.de/diso#hasSegment">
        <owl:inverseOf rdf:resource="https://purls.helmholtz-metadaten.de/diso#isSegmentOf"/>
        <rdfs:domain rdf:resource="https://purls.helmholtz-metadaten.de/diso#DiscretizedLine"/>
        <rdfs:range rdf:resource="https://purls.helmholtz-metadaten.de/diso#Segment"/>
        <rdfs:comment xml:lang="en">hasSegment represents the directed relation between discretized line and segment</rdfs:comment>
        <rdfs:label xml:lang="en">has segment</rdfs:label>
    </owl:ObjectProperty>
    


    <!-- https://purls.helmholtz-metadaten.de/diso#hasShapeFunction -->

    <owl:ObjectProperty rdf:about="https://purls.helmholtz-metadaten.de/diso#hasShapeFunction">
        <rdfs:domain rdf:resource="https://purls.helmholtz-metadaten.de/diso#DiscretizedLine"/>
        <rdfs:range rdf:resource="https://purls.helmholtz-metadaten.de/diso#ShapeFunction"/>
        <rdfs:comment xml:lang="en">hasShapeFunction represents the directed relation between discretized line and shape function</rdfs:comment>
        <rdfs:label xml:lang="en">has shape function</rdfs:label>
    </owl:ObjectProperty>
    


    <!-- https://purls.helmholtz-metadaten.de/diso#hasSlipDirection -->

    <owl:ObjectProperty rdf:about="https://purls.helmholtz-metadaten.de/diso#hasSlipDirection">
        <rdfs:subPropertyOf rdf:resource="https://purls.helmholtz-metadaten.de/diso#hasLatticeDirection"/>
        <rdfs:domain>
            <owl:Class>
                <owl:unionOf rdf:parseType="Collection">
                    <rdf:Description rdf:about="https://purls.helmholtz-metadaten.de/diso#SlipPlane"/>
                    <rdf:Description rdf:about="https://purls.helmholtz-metadaten.de/diso#SlipSystem"/>
                </owl:unionOf>
            </owl:Class>
        </rdfs:domain>
        <rdfs:range rdf:resource="https://purls.helmholtz-metadaten.de/diso#SlipDirection"/>
        <rdfs:comment xml:lang="en">hasSlipDirection represents the relationship  between Slip Plane or Slip system and Slip Direction they own.</rdfs:comment>
        <rdfs:label xml:lang="en">has slip direction</rdfs:label>
    </owl:ObjectProperty>
    


    <!-- https://purls.helmholtz-metadaten.de/diso#hasSlipPlane -->

    <owl:ObjectProperty rdf:about="https://purls.helmholtz-metadaten.de/diso#hasSlipPlane">
        <rdfs:subPropertyOf rdf:resource="https://purls.helmholtz-metadaten.de/diso#hasLatticePlane"/>
        <rdfs:range rdf:resource="https://purls.helmholtz-metadaten.de/diso#SlipPlane"/>
        <rdfs:comment xml:lang="en">hasSlipPlane represents the relationship between crystal structure and slip plane it owns.</rdfs:comment>
        <rdfs:label xml:lang="en">has slip plane</rdfs:label>
    </owl:ObjectProperty>
    


    <!-- https://purls.helmholtz-metadaten.de/diso#hasSlipPlaneNormal -->

    <owl:ObjectProperty rdf:about="https://purls.helmholtz-metadaten.de/diso#hasSlipPlaneNormal">
        <rdfs:domain>
            <owl:Class>
                <owl:unionOf rdf:parseType="Collection">
                    <rdf:Description rdf:about="https://purls.helmholtz-metadaten.de/diso#SlipPlane"/>
                    <rdf:Description rdf:about="https://purls.helmholtz-metadaten.de/diso#SlipSystem"/>
                </owl:unionOf>
            </owl:Class>
        </rdfs:domain>
        <rdfs:range rdf:resource="https://purls.helmholtz-metadaten.de/diso#SlipPlaneNormal"/>
        <rdfs:comment xml:lang="en">hasSlipPlaneNormal represents the relationship between a slip plane or slip system with slip plane normal.</rdfs:comment>
        <rdfs:label xml:lang="en">has slip plane normal</rdfs:label>
    </owl:ObjectProperty>
    


    <!-- https://purls.helmholtz-metadaten.de/diso#hasSlipSystem -->

    <owl:ObjectProperty rdf:about="https://purls.helmholtz-metadaten.de/diso#hasSlipSystem">
        <rdfs:range rdf:resource="https://purls.helmholtz-metadaten.de/diso#SlipSystem"/>
        <rdfs:comment xml:lang="en">hasSlipSystem represents the relationship between a crystal structure and slip system.</rdfs:comment>
        <rdfs:label xml:lang="en">has slip system</rdfs:label>
    </owl:ObjectProperty>
    


    <!-- https://purls.helmholtz-metadaten.de/diso#hasStartNode -->

    <owl:ObjectProperty rdf:about="https://purls.helmholtz-metadaten.de/diso#hasStartNode">
        <rdfs:subPropertyOf rdf:resource="https://purls.helmholtz-metadaten.de/diso#hasNode"/>
        <rdfs:domain rdf:resource="https://purls.helmholtz-metadaten.de/diso#Segment"/>
        <rdfs:range rdf:resource="https://purls.helmholtz-metadaten.de/diso#Node"/>
        <rdfs:comment xml:lang="en">Sub-property of hasNode that relates the segment with the start node</rdfs:comment>
        <rdfs:label xml:lang="en">has start node</rdfs:label>
    </owl:ObjectProperty>
    


    <!-- https://purls.helmholtz-metadaten.de/diso#isSegmentOf -->

    <owl:ObjectProperty rdf:about="https://purls.helmholtz-metadaten.de/diso#isSegmentOf">
        <rdfs:domain rdf:resource="https://purls.helmholtz-metadaten.de/diso#Segment"/>
        <rdfs:range rdf:resource="https://purls.helmholtz-metadaten.de/diso#DiscretizedLine"/>
        <rdfs:comment xml:lang="en">Inverse of hasSegment</rdfs:comment>
        <rdfs:label xml:lang="en">is segment of</rdfs:label>
    </owl:ObjectProperty>
    


    <!-- https://purls.helmholtz-metadaten.de/diso#movesOn -->

    <owl:ObjectProperty rdf:about="https://purls.helmholtz-metadaten.de/diso#movesOn">
        <rdfs:domain rdf:resource="https://purls.helmholtz-metadaten.de/diso#Dislocation"/>
        <rdfs:range rdf:resource="https://purls.helmholtz-metadaten.de/diso#SlipPlane"/>
        <rdfs:comment xml:lang="en">movesOn represents the relationship between dislocation and slip plane it moves on.</rdfs:comment>
        <rdfs:label xml:lang="en">moves on</rdfs:label>
    </owl:ObjectProperty>
    


    <!-- https://raw.githubusercontent.com/Materials-Data-Science-and-Informatics/dislocation-ontology/master/crystal-structure-ontology.owl#hasPositionVector -->

    <owl:ObjectProperty rdf:about="https://raw.githubusercontent.com/Materials-Data-Science-and-Informatics/dislocation-ontology/master/crystal-structure-ontology.owl#hasPositionVector">
        <rdfs:subPropertyOf rdf:resource="http://www.w3.org/2002/07/owl#topObjectProperty"/>
        <rdfs:range rdf:resource="https://purls.helmholtz-metadaten.de/cso#PositionVector"/>
        <rdfs:label xml:lang="en">has position vector</rdfs:label>
    </owl:ObjectProperty>
    


    <!-- 
    ///////////////////////////////////////////////////////////////////////////////////////
    //
    // Data properties
    //
    ///////////////////////////////////////////////////////////////////////////////////////
     -->

    


    <!-- https://purls.helmholtz-metadaten.de/diso#directionMillerIndice -->

    <owl:DatatypeProperty rdf:about="https://purls.helmholtz-metadaten.de/diso#directionMillerIndice">
        <rdfs:domain rdf:resource="https://purls.helmholtz-metadaten.de/diso#LatticeDirection"/>
        <rdfs:range rdf:resource="http://www.w3.org/2001/XMLSchema#string"/>
        <rdfs:comment xml:lang="en">directionMillerIndice represents Miller indice of lattice direction in string.</rdfs:comment>
        <rdfs:label xml:lang="en">direction miller indice</rdfs:label>
    </owl:DatatypeProperty>
    


    <!-- https://purls.helmholtz-metadaten.de/diso#familyDirectionMillerIndice -->

    <owl:DatatypeProperty rdf:about="https://purls.helmholtz-metadaten.de/diso#familyDirectionMillerIndice">
        <rdfs:domain rdf:resource="https://purls.helmholtz-metadaten.de/diso#FamilyOfCrystalDirection"/>
        <rdfs:range rdf:resource="http://www.w3.org/2001/XMLSchema#string"/>
        <rdfs:comment xml:lang="en">familyDirectionMillerIndice reprersent a set of miller indices of lattice direction in string.</rdfs:comment>
        <rdfs:label xml:lang="en">family direction miller indice</rdfs:label>
    </owl:DatatypeProperty>
    


    <!-- https://purls.helmholtz-metadaten.de/diso#familyPlaneMillerIndice -->

    <owl:DatatypeProperty rdf:about="https://purls.helmholtz-metadaten.de/diso#familyPlaneMillerIndice">
        <rdfs:domain rdf:resource="https://purls.helmholtz-metadaten.de/diso#FamilyOfCrystalPlane"/>
        <rdfs:range rdf:resource="http://www.w3.org/2001/XMLSchema#string"/>
        <rdfs:comment xml:lang="en">familyPlaneMillerIndice represents a set of Miller indice of lattice plane in string.</rdfs:comment>
        <rdfs:label xml:lang="en">family plane miller indice</rdfs:label>
    </owl:DatatypeProperty>
    


    <!-- https://purls.helmholtz-metadaten.de/diso#planeMillerIndice -->

    <owl:DatatypeProperty rdf:about="https://purls.helmholtz-metadaten.de/diso#planeMillerIndice">
        <rdfs:domain rdf:resource="https://purls.helmholtz-metadaten.de/diso#LatticePlane"/>
        <rdfs:range rdf:resource="http://www.w3.org/2001/XMLSchema#string"/>
        <rdfs:comment xml:lang="en">planeMillerIndice represents Miller indice of lattice plane in string.</rdfs:comment>
        <rdfs:label xml:lang="en">plane miller indice</rdfs:label>
    </owl:DatatypeProperty>
    


    <!-- https://purls.helmholtz-metadaten.de/diso#slipArea -->

    <owl:DatatypeProperty rdf:about="https://purls.helmholtz-metadaten.de/diso#slipArea">
        <rdfs:domain rdf:resource="https://purls.helmholtz-metadaten.de/diso#DiscretizedLine"/>
        <rdfs:range rdf:resource="http://www.w3.org/2001/XMLSchema#double"/>
    </owl:DatatypeProperty>
    


    <!-- 
    ///////////////////////////////////////////////////////////////////////////////////////
    //
    // Classes
    //
    ///////////////////////////////////////////////////////////////////////////////////////
     -->

    


    <!-- https://purls.helmholtz-metadaten.de/cso#CrystalStructure -->

    <owl:Class rdf:about="https://purls.helmholtz-metadaten.de/cso#CrystalStructure">
        <rdfs:subClassOf>
            <owl:Class>
                <owl:intersectionOf rdf:parseType="Collection">
                    <owl:Restriction>
                        <owl:onProperty rdf:resource="https://purls.helmholtz-metadaten.de/diso#hasSlipPlane"/>
                        <owl:someValuesFrom rdf:resource="https://purls.helmholtz-metadaten.de/diso#SlipPlane"/>
                    </owl:Restriction>
                    <owl:Restriction>
                        <owl:onProperty rdf:resource="https://purls.helmholtz-metadaten.de/diso#hasSlipPlane"/>
                        <owl:allValuesFrom rdf:resource="https://purls.helmholtz-metadaten.de/diso#SlipPlane"/>
                    </owl:Restriction>
                </owl:intersectionOf>
            </owl:Class>
        </rdfs:subClassOf>
        <rdfs:subClassOf>
            <owl:Class>
                <owl:intersectionOf rdf:parseType="Collection">
                    <owl:Restriction>
                        <owl:onProperty rdf:resource="https://purls.helmholtz-metadaten.de/diso#hasSlipSystem"/>
                        <owl:someValuesFrom rdf:resource="https://purls.helmholtz-metadaten.de/diso#SlipSystem"/>
                    </owl:Restriction>
                    <owl:Restriction>
                        <owl:onProperty rdf:resource="https://purls.helmholtz-metadaten.de/diso#hasSlipSystem"/>
                        <owl:allValuesFrom rdf:resource="https://purls.helmholtz-metadaten.de/diso#SlipSystem"/>
                    </owl:Restriction>
                </owl:intersectionOf>
            </owl:Class>
        </rdfs:subClassOf>
    </owl:Class>
    


    <!-- https://purls.helmholtz-metadaten.de/cso#Lattice -->

    <owl:Class rdf:about="https://purls.helmholtz-metadaten.de/cso#Lattice">
        <rdfs:subClassOf>
            <owl:Class>
                <owl:intersectionOf rdf:parseType="Collection">
                    <owl:Restriction>
                        <owl:onProperty rdf:resource="https://purls.helmholtz-metadaten.de/diso#hasLatticeDirection"/>
                        <owl:someValuesFrom rdf:resource="https://purls.helmholtz-metadaten.de/diso#LatticeDirection"/>
                    </owl:Restriction>
                    <owl:Restriction>
                        <owl:onProperty rdf:resource="https://purls.helmholtz-metadaten.de/diso#hasLatticeDirection"/>
                        <owl:allValuesFrom rdf:resource="https://purls.helmholtz-metadaten.de/diso#LatticeDirection"/>
                    </owl:Restriction>
                </owl:intersectionOf>
            </owl:Class>
        </rdfs:subClassOf>
        <rdfs:subClassOf>
            <owl:Class>
                <owl:intersectionOf rdf:parseType="Collection">
                    <owl:Restriction>
                        <owl:onProperty rdf:resource="https://purls.helmholtz-metadaten.de/diso#hasLatticePlane"/>
                        <owl:someValuesFrom rdf:resource="https://purls.helmholtz-metadaten.de/diso#LatticePlane"/>
                    </owl:Restriction>
                    <owl:Restriction>
                        <owl:onProperty rdf:resource="https://purls.helmholtz-metadaten.de/diso#hasLatticeDirection"/>
                        <owl:allValuesFrom rdf:resource="https://purls.helmholtz-metadaten.de/diso#LatticeDirection"/>
                    </owl:Restriction>
                </owl:intersectionOf>
            </owl:Class>
        </rdfs:subClassOf>
        <rdfs:subClassOf>
            <owl:Class>
                <owl:intersectionOf rdf:parseType="Collection">
                    <owl:Restriction>
                        <owl:onProperty rdf:resource="https://purls.helmholtz-metadaten.de/diso#hasLatticePoint"/>
                        <owl:someValuesFrom rdf:resource="https://purls.helmholtz-metadaten.de/diso#LatticePoint"/>
                    </owl:Restriction>
                    <owl:Restriction>
                        <owl:onProperty rdf:resource="https://purls.helmholtz-metadaten.de/diso#hasLatticePoint"/>
                        <owl:allValuesFrom rdf:resource="https://purls.helmholtz-metadaten.de/diso#LatticePoint"/>
                    </owl:Restriction>
                </owl:intersectionOf>
            </owl:Class>
        </rdfs:subClassOf>
        <rdfs:comment xml:lang="en">A lattice defines a periodic arrangement of one or more atoms.</rdfs:comment>
        <rdfs:comment xml:lang="en">A mathematical repsentation to represent the periodicity of a crystal.</rdfs:comment>
        <rdfs:label xml:lang="en">Lattice</rdfs:label>
    </owl:Class>
    


    <!-- https://purls.helmholtz-metadaten.de/cso#PositionVector -->

    <owl:Class rdf:about="https://purls.helmholtz-metadaten.de/cso#PositionVector">
        <rdfs:subClassOf rdf:resource="https://purls.helmholtz-metadaten.de/cso#Vector"/>
        <rdfs:comment xml:lang="en">Position vector is a Euclidean vector that represents the position of a point P in space in relation to an arbitrary reference origin O.</rdfs:comment>
        <rdfs:label xml:lang="en">Position Vector</rdfs:label>
    </owl:Class>
    


    <!-- https://purls.helmholtz-metadaten.de/cso#Vector -->

    <owl:Class rdf:about="https://purls.helmholtz-metadaten.de/cso#Vector">
        <rdfs:comment xml:lang="en">(Euclidean) vector used to represent quantities that both magnitude and direction.</rdfs:comment>
        <rdfs:label xml:lang="en">Vector</rdfs:label>
    </owl:Class>
    


    <!-- https://purls.helmholtz-metadaten.de/diso#BurgersVector -->

    <owl:Class rdf:about="https://purls.helmholtz-metadaten.de/diso#BurgersVector">
        <rdfs:subClassOf rdf:resource="https://purls.helmholtz-metadaten.de/cso#Vector"/>
        <rdfs:comment xml:lang="en">An elementary unit (length order of lattice parameter) of lattice translation.</rdfs:comment>
        <rdfs:comment xml:lang="en">The basic notion of Burgers vector comes from the closure failure of initially perfect lattice due to the existance of dislocation. The magnitude and direction of closure failure is characterized by Burgers vector.</rdfs:comment>
        <rdfs:label xml:lang="en">Burgers Vector</rdfs:label>
    </owl:Class>
    


    <!-- https://purls.helmholtz-metadaten.de/diso#DiscretizedLine -->

    <owl:Class rdf:about="https://purls.helmholtz-metadaten.de/diso#DiscretizedLine">
        <rdfs:subClassOf>
            <owl:Restriction>
                <owl:onProperty rdf:resource="https://purls.helmholtz-metadaten.de/diso#hasSegment"/>
                <owl:allValuesFrom rdf:resource="https://purls.helmholtz-metadaten.de/diso#Segment"/>
            </owl:Restriction>
        </rdfs:subClassOf>
        <rdfs:subClassOf>
            <owl:Restriction>
                <owl:onProperty rdf:resource="https://purls.helmholtz-metadaten.de/diso#hasShapeFunction"/>
                <owl:allValuesFrom rdf:resource="https://purls.helmholtz-metadaten.de/diso#ShapeFunction"/>
            </owl:Restriction>
        </rdfs:subClassOf>
        <rdfs:comment xml:lang="en">The numerical representation of dislocation line as a mathematical line, e.g. an oriented curve, is being discretized into the number of segments.</rdfs:comment>
        <rdfs:label xml:lang="en">Discretized Line</rdfs:label>
    </owl:Class>
    


    <!-- https://purls.helmholtz-metadaten.de/diso#Dislocation -->

    <owl:Class rdf:about="https://purls.helmholtz-metadaten.de/diso#Dislocation">
        <rdfs:subClassOf>
            <owl:Class>
                <owl:intersectionOf rdf:parseType="Collection">
                    <owl:Restriction>
                        <owl:onProperty rdf:resource="https://purls.helmholtz-metadaten.de/diso#hasBurgersVector"/>
                        <owl:someValuesFrom rdf:resource="https://purls.helmholtz-metadaten.de/diso#BurgersVector"/>
                    </owl:Restriction>
                    <owl:Restriction>
                        <owl:onProperty rdf:resource="https://purls.helmholtz-metadaten.de/diso#hasBurgersVector"/>
                        <owl:allValuesFrom rdf:resource="https://purls.helmholtz-metadaten.de/diso#BurgersVector"/>
                    </owl:Restriction>
                </owl:intersectionOf>
            </owl:Class>
        </rdfs:subClassOf>
        <rdfs:subClassOf>
            <owl:Class>
                <owl:intersectionOf rdf:parseType="Collection">
                    <owl:Restriction>
                        <owl:onProperty rdf:resource="https://purls.helmholtz-metadaten.de/diso#hasLineSense"/>
                        <owl:someValuesFrom rdf:resource="https://purls.helmholtz-metadaten.de/diso#LineSense"/>
                    </owl:Restriction>
                    <owl:Restriction>
                        <owl:onProperty rdf:resource="https://purls.helmholtz-metadaten.de/diso#hasLineSense"/>
                        <owl:allValuesFrom rdf:resource="https://purls.helmholtz-metadaten.de/diso#LineSense"/>
                    </owl:Restriction>
                </owl:intersectionOf>
            </owl:Class>
        </rdfs:subClassOf>
        <rdfs:subClassOf>
            <owl:Restriction>
                <owl:onProperty rdf:resource="https://purls.helmholtz-metadaten.de/diso#hasMathematicalRepresentation"/>
                <owl:someValuesFrom rdf:resource="https://purls.helmholtz-metadaten.de/diso#Line"/>
            </owl:Restriction>
        </rdfs:subClassOf>
        <rdfs:subClassOf>
            <owl:Restriction>
                <owl:onProperty rdf:resource="https://purls.helmholtz-metadaten.de/diso#movesOn"/>
                <owl:someValuesFrom rdf:resource="https://purls.helmholtz-metadaten.de/diso#SlipPlane"/>
            </owl:Restriction>
        </rdfs:subClassOf>
        <rdfs:comment xml:lang="en">A line object that is a boundary separating the regions on the slip plane which have undergone slip from those that have not.</rdfs:comment>
        <rdfs:comment xml:lang="en">Linear or one-dimensional defect around which some of the atoms are misaligned.</rdfs:comment>
        <rdfs:comment xml:lang="en">Presence of dislocation introduces local disturbance of the atomic-level geometry.</rdfs:comment>
        <rdfs:label xml:lang="en">Dislocation</rdfs:label>
        <rdfs:label xml:lang="de">Versetzung</rdfs:label>
    </owl:Class>
    


    <!-- https://purls.helmholtz-metadaten.de/diso#FamilyOfCrystalDirection -->

    <owl:Class rdf:about="https://purls.helmholtz-metadaten.de/diso#FamilyOfCrystalDirection">
        <rdfs:subClassOf>
            <owl:Restriction>
                <owl:onProperty rdf:resource="https://purls.helmholtz-metadaten.de/diso#familyDirectionMillerIndice"/>
                <owl:qualifiedCardinality rdf:datatype="http://www.w3.org/2001/XMLSchema#nonNegativeInteger">1</owl:qualifiedCardinality>
                <owl:onDataRange rdf:resource="http://www.w3.org/2001/XMLSchema#string"/>
            </owl:Restriction>
        </rdfs:subClassOf>
        <rdfs:comment xml:lang="en">a set of symmetrically equivalent directions in the lattice.</rdfs:comment>
        <rdfs:label xml:lang="en">Family of Crystal Direction</rdfs:label>
    </owl:Class>
    


    <!-- https://purls.helmholtz-metadaten.de/diso#FamilyOfCrystalPlane -->

    <owl:Class rdf:about="https://purls.helmholtz-metadaten.de/diso#FamilyOfCrystalPlane">
        <rdfs:subClassOf>
            <owl:Restriction>
                <owl:onProperty rdf:resource="https://purls.helmholtz-metadaten.de/diso#familyPlaneMillerIndice"/>
                <owl:qualifiedCardinality rdf:datatype="http://www.w3.org/2001/XMLSchema#nonNegativeInteger">1</owl:qualifiedCardinality>
                <owl:onDataRange rdf:resource="http://www.w3.org/2001/XMLSchema#string"/>
            </owl:Restriction>
        </rdfs:subClassOf>
        <rdfs:comment xml:lang="en">a set of symmetrically equivalent planes in the lattice.</rdfs:comment>
        <rdfs:label xml:lang="en">Family of Crystal Plane</rdfs:label>
    </owl:Class>
    


    <!-- https://purls.helmholtz-metadaten.de/diso#LatticeDirection -->

    <owl:Class rdf:about="https://purls.helmholtz-metadaten.de/diso#LatticeDirection">
        <rdfs:subClassOf rdf:resource="https://purls.helmholtz-metadaten.de/cso#Vector"/>
        <rdfs:subClassOf rdf:resource="https://purls.helmholtz-metadaten.de/diso#FamilyOfCrystalDirection"/>
        <rdfs:subClassOf>
            <owl:Class>
                <owl:intersectionOf rdf:parseType="Collection">
                    <owl:Restriction>
                        <owl:onProperty rdf:resource="https://purls.helmholtz-metadaten.de/diso#hasLatticePoint"/>
                        <owl:someValuesFrom rdf:resource="https://purls.helmholtz-metadaten.de/diso#LatticePoint"/>
                    </owl:Restriction>
                    <owl:Restriction>
                        <owl:onProperty rdf:resource="https://purls.helmholtz-metadaten.de/diso#hasLatticePoint"/>
                        <owl:allValuesFrom rdf:resource="https://purls.helmholtz-metadaten.de/diso#LatticePoint"/>
                    </owl:Restriction>
                </owl:intersectionOf>
            </owl:Class>
        </rdfs:subClassOf>
        <rdfs:subClassOf>
            <owl:Restriction>
                <owl:onProperty rdf:resource="https://purls.helmholtz-metadaten.de/diso#directionMillerIndice"/>
                <owl:qualifiedCardinality rdf:datatype="http://www.w3.org/2001/XMLSchema#nonNegativeInteger">1</owl:qualifiedCardinality>
                <owl:onDataRange rdf:resource="http://www.w3.org/2001/XMLSchema#string"/>
            </owl:Restriction>
        </rdfs:subClassOf>
        <rdfs:comment xml:lang="en">A direction inside the lattice that connecting two lattice points.</rdfs:comment>
        <rdfs:label xml:lang="en">Lattice Direction</rdfs:label>
    </owl:Class>
    


    <!-- https://purls.helmholtz-metadaten.de/diso#LatticePlane -->

    <owl:Class rdf:about="https://purls.helmholtz-metadaten.de/diso#LatticePlane">
        <rdfs:subClassOf rdf:resource="https://purls.helmholtz-metadaten.de/diso#FamilyOfCrystalPlane"/>
        <rdfs:subClassOf>
            <owl:Class>
                <owl:intersectionOf rdf:parseType="Collection">
                    <owl:Restriction>
                        <owl:onProperty rdf:resource="https://purls.helmholtz-metadaten.de/diso#hasLatticeDirection"/>
                        <owl:someValuesFrom rdf:resource="https://purls.helmholtz-metadaten.de/diso#LatticeDirection"/>
                    </owl:Restriction>
                    <owl:Restriction>
                        <owl:onProperty rdf:resource="https://purls.helmholtz-metadaten.de/diso#hasLatticeDirection"/>
                        <owl:allValuesFrom rdf:resource="https://purls.helmholtz-metadaten.de/diso#LatticeDirection"/>
                    </owl:Restriction>
                </owl:intersectionOf>
            </owl:Class>
        </rdfs:subClassOf>
        <rdfs:subClassOf>
            <owl:Class>
                <owl:intersectionOf rdf:parseType="Collection">
                    <owl:Restriction>
                        <owl:onProperty rdf:resource="https://purls.helmholtz-metadaten.de/diso#hasLatticePoint"/>
                        <owl:someValuesFrom rdf:resource="https://purls.helmholtz-metadaten.de/diso#LatticePoint"/>
                    </owl:Restriction>
                    <owl:Restriction>
                        <owl:onProperty rdf:resource="https://purls.helmholtz-metadaten.de/diso#hasLatticePoint"/>
                        <owl:allValuesFrom rdf:resource="https://purls.helmholtz-metadaten.de/diso#LatticePoint"/>
                    </owl:Restriction>
                </owl:intersectionOf>
            </owl:Class>
        </rdfs:subClassOf>
        <rdfs:subClassOf>
            <owl:Restriction>
                <owl:onProperty rdf:resource="https://purls.helmholtz-metadaten.de/diso#hasOrigin"/>
                <owl:allValuesFrom rdf:resource="https://purls.helmholtz-metadaten.de/diso#Origin"/>
            </owl:Restriction>
        </rdfs:subClassOf>
        <rdfs:subClassOf>
            <owl:Restriction>
                <owl:onProperty rdf:resource="https://purls.helmholtz-metadaten.de/diso#planeMillerIndice"/>
                <owl:qualifiedCardinality rdf:datatype="http://www.w3.org/2001/XMLSchema#nonNegativeInteger">1</owl:qualifiedCardinality>
                <owl:onDataRange rdf:resource="http://www.w3.org/2001/XMLSchema#string"/>
            </owl:Restriction>
        </rdfs:subClassOf>
        <rdfs:comment xml:lang="en">Lattice plane, forms an infinitely stretched plane (characterized through a plane normal) that cuts through lattice points such that again a regular arrangement of lattice points in the plane occurs.</rdfs:comment>
        <rdfs:label xml:lang="en">Lattice Plane</rdfs:label>
    </owl:Class>
    


    <!-- https://purls.helmholtz-metadaten.de/diso#LatticePoint -->

    <owl:Class rdf:about="https://purls.helmholtz-metadaten.de/diso#LatticePoint">
        <rdfs:subClassOf>
            <owl:Restriction>
                <owl:onProperty rdf:resource="https://raw.githubusercontent.com/Materials-Data-Science-and-Informatics/dislocation-ontology/master/crystal-structure-ontology.owl#hasPositionVector"/>
                <owl:allValuesFrom rdf:resource="https://purls.helmholtz-metadaten.de/cso#PositionVector"/>
            </owl:Restriction>
        </rdfs:subClassOf>
        <rdfs:comment xml:lang="en">Lattice points are the points where atoms or molecules are located</rdfs:comment>
        <rdfs:label xml:lang="en">Lattice Point</rdfs:label>
    </owl:Class>
    


    <!-- https://purls.helmholtz-metadaten.de/diso#Line -->

    <owl:Class rdf:about="https://purls.helmholtz-metadaten.de/diso#Line">
        <rdfs:subClassOf>
            <owl:Restriction>
                <owl:onProperty rdf:resource="https://purls.helmholtz-metadaten.de/diso#hasNumericalRepresentation"/>
                <owl:someValuesFrom rdf:resource="https://purls.helmholtz-metadaten.de/diso#DiscretizedLine"/>
            </owl:Restriction>
        </rdfs:subClassOf>
        <rdfs:comment xml:lang="en">Mathematical representation of dislocation as &apos;Line&apos;. An instance of mathematical representation of dislocation line is an oriented curve paramterized by its arc length.</rdfs:comment>
        <rdfs:label xml:lang="en">Line</rdfs:label>
    </owl:Class>
    


    <!-- https://purls.helmholtz-metadaten.de/diso#LineSense -->

    <owl:Class rdf:about="https://purls.helmholtz-metadaten.de/diso#LineSense">
        <rdfs:comment xml:lang="en">Sense that characterizes a directed line (has a start and an end).</rdfs:comment>
        <rdfs:label xml:lang="en">Line Sense</rdfs:label>
    </owl:Class>
    


    <!-- https://purls.helmholtz-metadaten.de/diso#Node -->

    <owl:Class rdf:about="https://purls.helmholtz-metadaten.de/diso#Node">
        <rdfs:subClassOf>
            <owl:Restriction>
                <owl:onProperty rdf:resource="https://raw.githubusercontent.com/Materials-Data-Science-and-Informatics/dislocation-ontology/master/crystal-structure-ontology.owl#hasPositionVector"/>
                <owl:allValuesFrom rdf:resource="https://purls.helmholtz-metadaten.de/cso#PositionVector"/>
            </owl:Restriction>
        </rdfs:subClassOf>
        <rdfs:comment xml:lang="en">Node of a segment</rdfs:comment>
        <rdfs:label xml:lang="en">Node</rdfs:label>
    </owl:Class>
    


    <!-- https://purls.helmholtz-metadaten.de/diso#Origin -->

    <owl:Class rdf:about="https://purls.helmholtz-metadaten.de/diso#Origin">
        <rdfs:subClassOf rdf:resource="https://purls.helmholtz-metadaten.de/cso#PositionVector"/>
        <rdfs:comment xml:lang="en">Origin is fixed point which is needed by vector to identify other points in the space relatives to its origin.</rdfs:comment>
        <rdfs:label xml:lang="en">Origin</rdfs:label>
    </owl:Class>
    


    <!-- https://purls.helmholtz-metadaten.de/diso#Segment -->

    <owl:Class rdf:about="https://purls.helmholtz-metadaten.de/diso#Segment">
        <rdfs:subClassOf>
            <owl:Restriction>
                <owl:onProperty rdf:resource="https://purls.helmholtz-metadaten.de/diso#hasNode"/>
                <owl:allValuesFrom rdf:resource="https://purls.helmholtz-metadaten.de/diso#Node"/>
            </owl:Restriction>
        </rdfs:subClassOf>
        <rdfs:subClassOf>
            <owl:Restriction>
                <owl:onProperty rdf:resource="https://purls.helmholtz-metadaten.de/diso#isSegmentOf"/>
                <owl:allValuesFrom rdf:resource="https://purls.helmholtz-metadaten.de/diso#DiscretizedLine"/>
            </owl:Restriction>
        </rdfs:subClassOf>
        <rdfs:comment xml:lang="en">A segment is a part of a line that is bounded by two distinct end points, and contains every point on the line that is between its endpoints.</rdfs:comment>
        <rdfs:label xml:lang="en">Segment</rdfs:label>
    </owl:Class>
    


    <!-- https://purls.helmholtz-metadaten.de/diso#ShapeFunction -->

    <owl:Class rdf:about="https://purls.helmholtz-metadaten.de/diso#ShapeFunction">
        <rdfs:comment xml:lang="en">The shape function is the function which interpolates the solution between the discrete values obtained at the mesh nodes. In the dicretized dislocation, the shape function detemines the shape of segment, ultimately determines the whole discretized line shape. Examples of shape function that is used to discretized the dislocation are, circular, elliptic, helical, linear, cubic, and quintic.</rdfs:comment>
        <rdfs:label xml:lang="en">Shape Function</rdfs:label>
    </owl:Class>
    


    <!-- https://purls.helmholtz-metadaten.de/diso#SlipDirection -->

    <owl:Class rdf:about="https://purls.helmholtz-metadaten.de/diso#SlipDirection">
        <rdfs:subClassOf rdf:resource="https://purls.helmholtz-metadaten.de/diso#LatticeDirection"/>
        <rdfs:comment xml:lang="en">The direction in the slip plane corresponding to one of the shortest lattice translation vectors.</rdfs:comment>
        <rdfs:label xml:lang="en">Slip Direction</rdfs:label>
    </owl:Class>
    


    <!-- https://purls.helmholtz-metadaten.de/diso#SlipPlane -->

    <owl:Class rdf:about="https://purls.helmholtz-metadaten.de/diso#SlipPlane">
        <rdfs:subClassOf rdf:resource="https://purls.helmholtz-metadaten.de/diso#LatticePlane"/>
        <rdfs:subClassOf>
            <owl:Class>
                <owl:intersectionOf rdf:parseType="Collection">
                    <owl:Restriction>
                        <owl:onProperty rdf:resource="https://purls.helmholtz-metadaten.de/diso#hasSlipDirection"/>
                        <owl:someValuesFrom rdf:resource="https://purls.helmholtz-metadaten.de/diso#SlipDirection"/>
                    </owl:Restriction>
                    <owl:Restriction>
                        <owl:onProperty rdf:resource="https://purls.helmholtz-metadaten.de/diso#hasSlipDirection"/>
                        <owl:allValuesFrom rdf:resource="https://purls.helmholtz-metadaten.de/diso#SlipDirection"/>
                    </owl:Restriction>
                </owl:intersectionOf>
            </owl:Class>
        </rdfs:subClassOf>
        <rdfs:subClassOf>
            <owl:Class>
                <owl:intersectionOf rdf:parseType="Collection">
                    <owl:Restriction>
                        <owl:onProperty rdf:resource="https://purls.helmholtz-metadaten.de/diso#hasSlipPlaneNormal"/>
                        <owl:someValuesFrom rdf:resource="https://purls.helmholtz-metadaten.de/diso#SlipPlaneNormal"/>
                    </owl:Restriction>
                    <owl:Restriction>
                        <owl:onProperty rdf:resource="https://purls.helmholtz-metadaten.de/diso#hasSlipPlaneNormal"/>
                        <owl:allValuesFrom rdf:resource="https://purls.helmholtz-metadaten.de/diso#SlipPlaneNormal"/>
                    </owl:Restriction>
                </owl:intersectionOf>
            </owl:Class>
        </rdfs:subClassOf>
        <rdfs:comment xml:lang="en">Slip plane is normally the plane with the highest density of atoms, i.e. those which are most widely spaced.</rdfs:comment>
        <rdfs:comment xml:lang="en">The crystallographic plane along which the dislocation line traverses.</rdfs:comment>
        <rdfs:label xml:lang="en">Slip Plane</rdfs:label>
    </owl:Class>
    


    <!-- https://purls.helmholtz-metadaten.de/diso#SlipPlaneNormal -->

    <owl:Class rdf:about="https://purls.helmholtz-metadaten.de/diso#SlipPlaneNormal">
        <rdfs:subClassOf rdf:resource="https://purls.helmholtz-metadaten.de/cso#Vector"/>
        <rdfs:subClassOf>
            <owl:Restriction>
                <owl:onProperty rdf:resource="https://purls.helmholtz-metadaten.de/diso#directionMillerIndice"/>
                <owl:qualifiedCardinality rdf:datatype="http://www.w3.org/2001/XMLSchema#nonNegativeInteger">1</owl:qualifiedCardinality>
                <owl:onDataRange rdf:resource="http://www.w3.org/2001/XMLSchema#string"/>
            </owl:Restriction>
        </rdfs:subClassOf>
        <rdfs:comment xml:lang="en">Unit normal vector of slip planes</rdfs:comment>
        <rdfs:label xml:lang="en">Slip Plane Normal</rdfs:label>
    </owl:Class>
    


    <!-- https://purls.helmholtz-metadaten.de/diso#SlipSystem -->

    <owl:Class rdf:about="https://purls.helmholtz-metadaten.de/diso#SlipSystem">
        <rdfs:subClassOf>
            <owl:Class>
                <owl:intersectionOf rdf:parseType="Collection">
                    <owl:Restriction>
                        <owl:onProperty rdf:resource="https://purls.helmholtz-metadaten.de/diso#hasSlipDirection"/>
                        <owl:someValuesFrom rdf:resource="https://purls.helmholtz-metadaten.de/diso#SlipDirection"/>
                    </owl:Restriction>
                    <owl:Restriction>
                        <owl:onProperty rdf:resource="https://purls.helmholtz-metadaten.de/diso#hasSlipDirection"/>
                        <owl:allValuesFrom rdf:resource="https://purls.helmholtz-metadaten.de/diso#SlipDirection"/>
                    </owl:Restriction>
                </owl:intersectionOf>
            </owl:Class>
        </rdfs:subClassOf>
        <rdfs:subClassOf>
            <owl:Class>
                <owl:intersectionOf rdf:parseType="Collection">
                    <owl:Restriction>
                        <owl:onProperty rdf:resource="https://purls.helmholtz-metadaten.de/diso#hasSlipPlaneNormal"/>
                        <owl:someValuesFrom rdf:resource="https://purls.helmholtz-metadaten.de/diso#SlipPlaneNormal"/>
                    </owl:Restriction>
                    <owl:Restriction>
                        <owl:onProperty rdf:resource="https://purls.helmholtz-metadaten.de/diso#hasSlipPlaneNormal"/>
                        <owl:allValuesFrom rdf:resource="https://purls.helmholtz-metadaten.de/diso#SlipPlaneNormal"/>
                    </owl:Restriction>
                </owl:intersectionOf>
            </owl:Class>
        </rdfs:subClassOf>
        <rdfs:comment xml:lang="en">Slip system is defined as the set of slip planes with the same unit normal vector and the same slip direction.</rdfs:comment>
        <rdfs:label xml:lang="en">Slip System</rdfs:label>
    </owl:Class>
</rdf:RDF>



<!-- Generated by the OWL API (version 4.5.9.2019-02-01T07:24:44Z) https://github.com/owlcs/owlapi -->

